SMT/HOTyping.lean
@@ -2,6 +2,6 @@ import SMT.HOTyping.Rules
 
 namespace SMT.PHOAS
 
-abbrev WellTyped.{u} {𝒱 : Type u} [DecidableEq 𝒱] [Inhabited 𝒱] (t : Term 𝒱) := Σ' (Γ : TypeContext 𝒱) (τ : SMTType), Γ ⊢ t : τ
+abbrev WellTyped.{u} {𝒱 : Type u} [DecidableEq 𝒱] [Inhabited 𝒱] (t : Term 𝒱) := Σ' (Γ : TypeContext 𝒱) (τ : SMTType), Γ ⊢ˢ' t : τ
 
 end SMT.PHOAS
